@prefix lv2:    <http://lv2plug.in/ns/lv2core#> .
@prefix mod:    <http://moddevices.com/ns/mod#> .
@prefix owl:    <http://www.w3.org/2002/07/owl#> .
@prefix pprops: <http://lv2plug.in/ns/ext/port-props#> .
@prefix rdf:    <http://www.w3.org/1999/02/22-rdf-syntax-ns#> .
@prefix rdfs:   <http://www.w3.org/2000/01/rdf-schema#> .
@prefix xsd:    <http://www.w3.org/2001/XMLSchema#> .

<http://moddevices.com/ns/mod>
    a owl:Ontology ;
    rdfs:seeAlso <mod.doap.ttl> ;
    lv2:documentation """
<p>
This is a vocabulary for describing extra plugin data specific to MOD software and devices.
</p>
""" .

mod:brand
    a rdf:Property ,
        owl:DatatypeProperty ;
    rdfs:label "brand" ;
    rdfs:range xsd:string ;
    rdfs:comment "A short plugin brand name. Maximum of 11 characters" .

mod:label
    a rdf:Property ,
        owl:DatatypeProperty ;
    rdfs:label "label" ;
    rdfs:range xsd:string ;
    rdfs:comment "A short plugin label. Maximum of 16 characters" .

mod:default
    a rdf:Property ,
        owl:DatatypeProperty ,
        owl:FunctionalProperty ;
    rdfs:label "default" ;
    rdfs:seeAlso lv2:default ;
    rdfs:comment "A custom default value specific to MOD devices, used in place of lv2:default." .

mod:minimum
    a rdf:Property ,
        owl:DatatypeProperty ,
        owl:FunctionalProperty ;
    rdfs:label "minimum" ;
    rdfs:seeAlso lv2:minimum ;
    rdfs:comment "A custom minimum value specific to MOD devices, used in place of lv2:minimum." .

mod:maximum
    a rdf:Property ,
        owl:DatatypeProperty ,
        owl:FunctionalProperty ;
    rdfs:label "maximum" ;
    rdfs:seeAlso lv2:maximum ;
    rdfs:comment "A custom maximum value specific to MOD devices, used in place of lv2:maximum." .

mod:rangeSteps
    a rdf:Property ;
    rdfs:domain lv2:Port ;
    rdfs:range xsd:nonNegativeInteger ;
    rdfs:label "number of value steps" ;
    rdfs:seeAlso pprops:rangeSteps ;
    rdfs:comment "A custom rangeSteps value specific to MOD devices, used in place of pprops:rangeSteps." .

mod:builderVersion
    a rdf:Property ,
        owl:DatatypeProperty ,
        owl:FunctionalProperty ;
    rdfs:label "builder version" ;
    rdfs:comment "The version of the MOD cloud builder used to compile a plugin." .

mod:releaseNumber
    a rdf:Property ,
        owl:DatatypeProperty ,
        owl:FunctionalProperty ;
    rdfs:label "release number" ;
    rdfs:comment "The MOD build release number of a bundle. This number is auto-incremented everytime the cloud rebuilds or updates the plugin." .

mod:tapTempo
    a lv2:PortProperty ;
    rdfs:label "tap tempo" ;
    rdfs:comment "Indicates that the port is suitable for a MOD foot-switch addressing, by using hardware-side tap tempo. Please note that a unit of time is required on the port for tap tempo to work properly. The supported unit types are 'ms', 's', 'Hz' and 'bpm'."

mod:notStompboxCapable
    a lv2:Feature ;
    rdfs:label "not stompbox capable" ;
    lv2:documentation """
<p>
Indicates that the plugin is not suitable for use in the MOD Stompbox mode.<br/>
Plugins are assumed to be suitable for Stompbox mode by default, and MUST provide this as an optional feature in case that's not true.
</p>
""" .
